floyd/Funspec_old_Notation.v
@@ -1,4 +1,7 @@
-Require Export VST.floyd.funspec_old.
+(* Warning! Old-style funspecs are not well supported in VST 3.x. If you really want to use
+   them, you can uncomment the lines below, but do so at your own risk -- calls to them may
+   fail, or they may cause start_function to run forever. *)
+(*Require Export VST.floyd.funspec_old.*)
 
-Global Close Scope funspec_scope.
-Global Open Scope old_funspec_scope.
+(*Global Close Scope funspec_scope.
+Global Open Scope old_funspec_scope.*)
