sha/verif_sha_final.v
@@ -48,7 +48,7 @@ rewrite H7. clear H7.
 subst r_h r_Nh r_Nl r_num.
 forward. (* p = c->data;  *)
 simpl (temp _p _).
-assert_PROP (field_address t_struct_SHA256state_st [StructField _data] c = offset_val (320/8) c).
+assert_PROP (field_address t_struct_SHA256state_st [StructField _data] c = offset_val 40 c).
  entailer!.
 rewrite <- H0; clear H0.
 forward. (* n = c->num; *)
